Fix ordset

examples/simple.ml
@@ -1,8 +1,9 @@
+
+let f = FStar_OrdSet.intersect
 module User = struct
   type t = { username : string }
 
-  let equal _a _b = false
-  (* String.equal a.username b.username *)
+  let equal a b = String.equal a.username b.username
 
   let pp ppf v = Format.pp_print_string ppf v.username
 end
@@ -13,7 +14,9 @@ let alice = User.{ username = "Alice" }
 let bob = User.{ username = "Bob" }
 let charlie = User.{ username = "Charlie" }
 let meredith = User.{ username = "Meredith" }
-let map = Users.v alice [ bob ] |> Users.add charlie [ meredith; bob ]
+let map = Users.v alice [ alice; bob ] 
+          |> Users.add charlie [ alice; meredith; bob ]
+          |> Users.add meredith [ alice ]
 let owners = Users.owners map
 let ef = Users.effective_readers map
 
@@ -23,19 +26,3 @@ let () =
   print_endline "\nEffective Reader Set:";
   List.iter (Format.printf "%a\n%!" User.pp) ef
 
-(* Using Monad like type *)
-
-let map2 = Users.v meredith [ alice ]
-
-let v =
-  let module M = Users.Monad in
-  let open M.Syntax in
-  let* v1 = M.return map "Secret " in
-  let+ v2 = M.return map2 "Data" in
-  v1 ^ v2
-
-let () =
-  print_endline "Owners v:";
-  List.iter
-    (Format.printf "%a\n%!" User.pp)
-    (Users.owners (Users.Monad.label v))
