src/ml/difc.ml
@@ -1,38 +1,54 @@
 (* Raw FStar generated code *)
 module Low_level = Difc_fstar
+module S = FStar_OrdSet
 module M = FStar_OrdMap
 
 module type Principal = sig
   type t
 
   val equal : t -> t -> bool
+
+  val pp : Format.formatter -> t -> unit
 end
 
 module Make (P : Principal) = struct
-  type t = (P.t, P.t list, unit) FStar_OrdMap.ordmap
+  type t = (P.t, (P.t, unit) S.ordset, unit) FStar_OrdMap.ordmap
 
   (* Don't expose! *)
   let empty = M.empty P.equal
-  let add o v = M.update P.equal o v
+  let add o v = M.update P.equal o (List.sort compare v)
   let v owner readers = empty |> add owner readers
   let owners v = Low_level.owners P.equal v
   let effective_readers v = Low_level.effective_readers P.equal v
+  let pp_pair f1 f2 =
+    (fun ppf (a, b) -> Format.fprintf ppf "(%a, %a)" f1 a f2 b)
+  
+  let pp ppf (f : t) =
+    let owners = M.dom P.equal f in
+    let rec fold acc = function
+      | [] -> List.rev acc
+      | o :: os ->
+      match M.select P.equal o f with
+      | Some rs ->
+        fold ((o, S.as_list P.equal rs) :: acc) os
+      | None -> fold acc os
+    in
+    let lst = fold [] owners in
+    Format.fprintf ppf "%a" Format.(pp_print_list (pp_pair P.pp (pp_print_list P.pp))) lst
 
   module Monad = struct
-    type v = t
     type 'a t = ('a, P.t, unit) Difc_fstar_monad.difc_monad
 
     let label (v : 'a t) = v.label
-    let return (l : v) (v : 'a) : 'a t = Difc_fstar_monad.return P.equal l v
+    let return l (v : 'a) : 'a t = Difc_fstar_monad.return P.equal l v
 
     let bind (fn : 'a -> 'b t) (v : 'a t) : 'b t =
       Difc_fstar_monad.bind P.equal fn v
-
-    let map (fn : 'a -> 'b) (v : 'a t) : 'b t =
-      Difc_fstar_monad.map P.equal fn v
-
-    let map_pair (f : 'a -> 'b -> 'c) (m : 'a t) (n : 'b t) : 'c t =
-      Difc_fstar_monad.map_pair P.equal f m n
+    
+    let map (fn : 'a -> 'b) (v : 'a t) : 'b t = Difc_fstar_monad.map P.equal fn v
+      
+    let pair v1 v2 =
+      Difc_fstar_monad.pair P.equal v1 v2
 
     module Syntax = struct
       let ( let+ ) v f = map f v
