src/ml/difc.mli
@@ -1,0 +1,46 @@
+
+(* Raw FStar generated code *)
+module Low_level = Difc_fstar
+module M = FStar_OrdMap
+
+module type Principal = sig
+  type t
+
+  val equal : t -> t -> bool
+  
+  val pp : Format.formatter -> t -> unit
+end
+
+module Make (P : Principal) : sig 
+  type t
+
+  val pp : Format.formatter -> t -> unit
+
+  val v : P.t -> P.t list -> t
+  (* A new label with a single owner and set of readers *)
+
+  val add : P.t -> P.t list -> t -> t
+
+  val owners : t -> P.t list
+
+  val effective_readers : t -> P.t list
+
+  module Monad : sig
+    type label := t
+    type 'a t
+    (** Labelled values *)
+
+    val label : 'a t -> label
+
+    val return : label -> 'a -> 'a t
+
+    val bind : ('a -> 'b t) -> 'a t -> 'b t
+    val map : ('a -> 'b) -> 'a t -> 'b t
+    val pair : 'a t -> 'b t -> ('a * 'b) t
+
+    module Syntax : sig
+     val ( let* ) : 'a t -> ('a -> 'b t) -> 'b t
+     val ( let+ ) : 'a t -> ('a -> 'b) -> 'b t
+    end
+  end
+end
