README.md
@@ -4,4 +4,59 @@ difc*
 Formalisation of DIFC 
 ([A Decentralized Model for Information Flow Control](https://www.cs.cornell.edu/andru/papers/iflow-sosp97/paper.html)) using FStar.
 
+Create a custom DIFC model with a user-defined principal.
 
+```ocaml
+module User = struct
+  type t = { username : string }
+
+  let equal a b = String.equal a.username b.username
+
+  let pp ppf v = Format.pp_print_string ppf v.username
+end
+
+module Users = Difc.Make (User)
+module M = Users.Monad
+open M.Syntax
+
+(* Some users *)
+let anil = User.{ username = "Anil" }
+let ryan = User.{ username = "Ryan" }
+let jessica = User.{ username = "Jessica" }
+let michael = User.{ username = "Michael" }
+let maddy = User.{ username = "Maddy" }
+let patrick = User.{ username = "Patrick" }
+```
+
+Track labels using the built-in operators.
+
+```ocaml
+# let ryans_label = Users.v ryan [ michael; anil ];;
+val ryans_label : Users.t = <abstr>
+# let jessicas_label = Users.v jessica [ maddy; anil ];;
+val jessicas_label : Users.t = <abstr>
+# let patricks_label = Users.v patrick [ ryan; anil ];;
+val patricks_label : Users.t = <abstr>
+```
+
+Combine data and restrict the resulting label.
+
+```ocaml
+# let v =
+    let* patricks_data = M.return patricks_label "Super " in
+    let* ryans_data = M.return ryans_label " secret " in
+    let+ jessicas_data = M.return jessicas_label "data" in 
+    patricks_data ^ ryans_data ^ jessicas_data
+val v : string M.t = <abstr>
+```
+
+We can look at the new data's label.
+
+```ocaml
+# M.label v |> Users.owners
+- : User.t list =
+[{User.username = "Patrick"}; {User.username = "Ryan"};
+ {User.username = "Jessica"}]
+# M.label v |> Users.effective_readers
+- : User.t list = [{User.username = "Anil"}]
+```
